leyland work on Isabelle/GST

src/Founder/Test.thy
@@ -1,130 +1,71 @@
 theory Test
-  imports ZFC_in_HOL_Bootstrap 
-    "../Ordinal/Model/OrdRec_Model" "../GZF/KPair"  
-   
+  imports  "../Ordinal/Model/OrdRec_Model" ZFC_in_HOL_Bootstrap      
 begin 
-ML_file \<open>../ModelKit/Tools/build_model_operator.ML\<close> 
 
-ML \<open>val GZF_OPair_ts = 
-   [\<^term>\<open>is_kpair :: V \<Rightarrow> bool\<close>, \<^term>\<open>kpair :: V \<Rightarrow> V \<Rightarrow> V\<close>,
-    \<^term>\<open>SetMem :: V \<Rightarrow> bool\<close>, \<^term>\<open>GZF_default :: V\<close>]\<close>
-
-setup \<open>mk_instantiation \<^type_name>\<open>V\<close> \<^class>\<open>OPair\<close> GZF_OPair_ts @{thm GZF_OPair}\<close>
-
-instance V :: Function sorry
-instance V :: CartProd sorry
+ML_file \<open>../ModelKit/Tools/model_implementation.ML\<close>
 instance V :: Tagging ..
- 
-(*cols should be a list of (i, t) where i is a term denoting an ordinal,
-  and is a term of type D \<Rightarrow> bool *)
-(*all of the stuff below needs a major refactor*)
-ML \<open>fun mk_excluded typ cols =
-  let
-    val (i,b) = (Bound 1, Bound 0) 
-    val ex_seq = map (fn (ord, t) => (ord, betapply (t,b))) cols
-    val body = mk_ord_seq \<^typ>\<open>bool\<close> i \<^term>\<open>True\<close> ex_seq
-    in Term.abs ("i", typ) (Term.abs ("b", typ) body) end\<close>
 
-ML \<open>fun mk_slot_typs typ seq =
-  let
-    val any = Const ("Soft_Types.Any", typ --> \<^typ>\<open>bool\<close>)
-    val body = mk_ord_seq (typ --> \<^typ>\<open>bool\<close>) (Bound 0) any seq
-  in (Term.abs ("i", typ) body) end\<close>
+lemma if_cases : 
+  assumes "Q \<Longrightarrow> P x" "\<not> Q \<Longrightarrow> P y"
+  shows "P (if Q then x else y)"
+  using assms by auto
 
-ML \<open>fun excluded_rule typ (exname, exdef_thm, ex_trm) (n, otrm, pred) lthy = 
-  let 
-    val b = Free ("b",typ)
-    val iff = HOLogic.mk_Trueprop ((\<^term>\<open>iff\<close> $  
-         (betapplys (ex_trm, [otrm, b]))) $ betapply (pred, b))
-    val thm_name = exname ^ "_" ^ Int.toString n
-    val state = Proof.theorem NONE (after_qed (Binding.name thm_name, [])) 
-                [[(iff,[])]] lthy
-    val state' = Proof.unfolding [[([exdef_thm, if_thm n], [])]] state
-  in
-    Proof.global_default_proof state'
-  end\<close>
-
-ML \<open>fun slottype_rule (iden, def_thm, trm) (n, otrm, styp) lthy = 
-  let 
-    val eq = HOLogic.mk_Trueprop (HOLogic.mk_eq (betapply (trm, otrm), styp))
-    val thm_name = iden ^ "_" ^ Int.toString n
-    val state = Proof.theorem NONE (after_qed (Binding.name thm_name, [])) 
-                [[(eq,[])]] lthy
-    val state' = Proof.unfolding [[([def_thm, if_thm n], [])]] state
-  in
-    Proof.global_default_proof state'
-  end\<close>
-
-ML \<open>fun create_excluded_op typ ts lthy = 
-  let
-    val ex_name = "Excluded_" ^ last_field (fst (Term.dest_Type typ))
-    val ords = ordinal_list typ (length ts - 1)
-    val ex_trm = mk_excluded typ (ords ~~ ts)
-    val ((trm, (_,thm)), lthy) = make_defn_all ex_name ex_trm NoSyn lthy
-    val ints_ords_preds = (0 upto (length ords - 1) ~~ (ords ~~ ts))
-    fun add_rule ((n,(i,p)),lthy) = excluded_rule typ (ex_name, thm, trm) (n,i,p) lthy
-  in
-    List.foldl add_rule lthy ints_ords_preds
-  end\<close>
-
-ML \<open>fun create_slot_typ_op typ styps lthy = 
-  let
-    val iden = "\<alpha>_" ^ last_field (fst (Term.dest_Type typ))
-    val ords = ordinal_list typ (length styps - 1)
-    val ex_trm = mk_slot_typs typ (ords ~~ styps)
-    val ((trm, (_,thm)), lthy) = make_defn_all iden ex_trm NoSyn lthy
-    val ints_ords_preds = (0 upto (length ords - 1) ~~ (ords ~~ styps))
-    fun add_rule ((n,(i,p)),lthy) = slottype_rule (iden, thm, trm) (n,i,p) lthy
-  in
-    List.foldl add_rule lthy ints_ords_preds
-  end\<close>
-
-ML \<open>fun get_tags ms = (map (get_mcomp_tag) 
-                o filter (fn mcomp {variant,...} => Option.isSome variant))
-                  (resolve_mdeps ms)\<close>
-
-ML \<open>fun defn_tags typ ms lthy = 
-    let
-      val tag_idens = get_tags ms
-      val ords = ordinal_list typ (length tag_idens - 1)
-      val defs = map (fn (iden,trm) => 
-        (iden ^ "_" ^ last_field (fst (Term.dest_Type typ)),trm, NoSyn)) (tag_idens ~~ ords)
-    in make_defns lthy defs end\<close>
-
-ML \<open>
-fun model_implementation typ ms ex_preds styps =
-    (defn_tags typ ms)
-  o (create_variants_op typ ms) 
-  o (create_excluded_op typ ex_preds)
-  o (create_slot_typ_op typ styps)\<close>
-
-instantiation V :: ModelBase' begin
+instantiation V :: ModelBase begin
   (*Call Variants: TierImplementation, change Ordinal_default to \<emptyset> *)
   local_setup \<open>model_implementation \<^typ>\<open>V\<close> [ordrec_model] 
     [\<^term>\<open>\<lambda>x :: V. False\<close>, \<^term>\<open>\<lambda>x :: V. False\<close>]
     [\<^term>\<open>Set :: V \<Rightarrow> bool\<close>, \<^term>\<open>Ord :: V \<Rightarrow> bool\<close>]\<close>
 
-  thm Variants_V_def Excluded_V_def set_V_def ord_V_def
+  thm Variants_V_def Excluded_V_def
   thm Variants_V_0 Variants_V_0_zero Variants_V_0_succ Variants_V_0_lim
   thm Variants_V_1 Variants_V_1_zero Variants_V_1_succ Variants_V_1_lim 
   thm Excluded_V_0 Excluded_V_1
   
-  instance 
-  proof (intro_classes)
+  instance proof (intro_classes)
     show "Variants : (\<Pi> i::V:Tag. nonLimit \<rightarrow> Set \<rightarrow> SetOf (\<alpha> i))"
     proof (rule depfunI, rule funI, rule funI)
       fix i :: V and j :: V and x :: V 
-      assume "i : Tag" "j : nonLimit" "x : Set"
-      hence "i : Ordinal_class.Ord" "i < \<omega>" 
-        using tagD by auto
+      assume "i : Tag" "j : nonLimit" and x :"x : Set"
+      hence "i : Ord" "i < \<omega>" and j : "j : Ord"  
+        using tagD nonlimit_ord by auto
         
-      have "Variants 0 j x : SetOf Set"  
-        unfolding Variants_V_0
-      proof (rule case_ordE[OF nonlimit_ord[OF \<open>j : nonLimit\<close>]])
       show "Variants i j x : SetOf (\<alpha> i)"
-     
- end
-instance V :: GZF_Model sorry
+        unfolding Variants_V_def \<alpha>_V_def 
+        by (rule iffD2[OF if_split], rule, rule,
+            use gzf_model_case_typ[OF j x] 
+                ord_model_case_typ[OF j] emp_setof in auto)
+    qed
+
+    show "Variants : (\<Pi> (i::V) : Tag. Limit \<rightarrow> Function \<rightarrow> SetOf (\<alpha> i)) "
+    proof (rule depfunI, rule funI, rule funI)
+      fix i :: V and u :: V and f :: V 
+      assume "i : Tag" "u : Limit" "f : Function" 
+      show "Variants i u f : SetOf (\<alpha> i)"
+        unfolding Variants_V_def case_ord_lim[OF \<open>u : Limit\<close>]
+      proof (rule if_cases[OF _ if_cases], rule emp_setof)
+        assume i:"i = succ 0"
+        show "{u} : SetOf (\<alpha> i)"
+          unfolding i \<alpha>_V_1
+          using sng_setof[OF ord_setmem] 
+            limit_ord[OF \<open>u : Limit\<close>] by auto
+      next
+        show "\<emptyset> : SetOf (\<alpha> i)"
+          using emp_setof .
+      qed
+    qed
+  qed
+end
+
+instantiation V :: GZF_Model 
+begin
+
+  definition mdefault_V :: V where
+    "mdefault_V \<equiv> <set_V,\<emptyset>>"
+  thm Variants_V_0_zero
+  instance proof (intro_classes)
+    show "(mdefault::V) : M"
+        
+end
 instance V :: Ordinal_Model sorry
 instance V :: OrdRec_Model sorry
 
