src/Relations/Relations.thy
@@ -7,7 +7,7 @@ context BinRel begin
 thm mkrel_typ field_typ
 thm rel ext field_iff
 
-lemmas mkrel_binrel = funE[OF depfunE[OF depfunE[OF mkrel_typ]]]
+lemmas mkrel_binrel = funE[OF funE[OF funE[OF mkrel_typ]] anyI]
 lemmas field_set = funE[OF field_typ]
 
 lemma brelmemI1 :
@@ -44,9 +44,11 @@ definition FuncRel :: "'a \<Rightarrow> bool"
   where "FuncRel \<equiv> BinRel \<triangle> (\<lambda>r. \<forall>a b c. app r a b \<and> app r a c \<longrightarrow> b = c)"
 
 definition FuncRelPred 
-  where "FuncRelPred x \<equiv> ReplPred x \<triangle> (\<lambda>P. BinRelPred x (Repl x P) P)"
+  where "FuncRelPred s P \<equiv> \<forall>x : BinRelMem. x \<in> s \<longrightarrow> (\<exists>\<^sub>\<le>\<^sub>1 y : BinRelMem. P x y)"
 
-definition mk_funrel where "mk_funrel x P \<equiv> mkrel x (Repl x P) P"
+definition mk_funrel 
+  where "mk_funrel x P \<equiv> 
+    mkrel {a \<in> x | a : BinRelMem} (Repl x (\<lambda>a b. a : BinRelMem \<and> b : BinRelMem \<and> P a b)) P"
 
 interpretation Function
   where Function = FuncRel
@@ -72,75 +74,104 @@ qed
 
 lemmas relmem_setmem = subtypE[OF relmem_setmem_subtyp]
 
-lemma frelpred_replpred :
-  assumes "P : FuncRelPred x"
-  shows "P : ReplPred x" 
-   using assms unfolding FuncRelPred_def 
-   by unfold_typs
-
+(* 
 lemma frelpred_brelpred :
   assumes "P : FuncRelPred x"
   shows "P : BinRelPred x (Repl x P)" 
-   using assms unfolding FuncRelPred_def 
-   by unfold_typs
+   using assms unfolding FuncRelPred_def *) 
+   (* by unfold_typs *)
+
+lemma frelpred_replpred : 
+  assumes "P : FuncRelPred x"
+  shows "(\<lambda>a b. a : BinRelMem \<and> b : BinRelMem \<and> P a b) : ReplPred x"
+proof (rule replpredI, unfold tuniq_def Uniq_def, auto)
+  fix a b b' assume
+    "a \<in> x" "a : BinRelMem" "b : BinRelMem" "b' : BinRelMem" "P a b" "P a b'"
+  thus "b = b'"  
+    using assms 
+    unfolding FuncRelPred_def has_ty_def tall_def tuniq_def Uniq_def
+    by auto
+qed
+
+lemma mk_funrel_binrel : 
+  assumes x : "x : Set" and P : "P : FuncRelPred x"
+  shows "mk_funrel x P : BinRel"
+  unfolding mk_funrel_def
+  using mkrel_binrel[OF collect_set[OF x] repl_set[OF x frelpred_replpred[OF P]]] . 
 
 lemma mkfun_rel_iff :
   assumes x : "x : Set" and P : "P : FuncRelPred x" 
-  shows "\<forall>a b. app (mk_funrel x P) a b \<longleftrightarrow> (a \<in> x \<and> b \<in> Repl x P \<and> P a b)"
+  shows "\<forall>a b. app (mk_funrel x P) a b \<longleftrightarrow> 
+    (a \<in> x \<and> P a b \<and> a : BinRelMem \<and> b : BinRelMem)"
 proof -
-  have "Repl x P : Set" "P : BinRelPred x (Repl x P)"  
-    using repl_set[OF x frelpred_replpred[OF P]] frelpred_brelpred[OF P] by auto
-  thus "\<forall>a b. app (mk_funrel x P) a b \<longleftrightarrow> (a \<in> x \<and> b \<in> Repl x P \<and> P a b)"
-    using rel \<open>x : Set\<close> unfolding mk_funrel_def tall_def by auto
+  have r_set:"Repl x (\<lambda>a b. a : BinRelMem \<and> b : BinRelMem \<and> P a b) : Set"  
+    using repl_set[OF x frelpred_replpred[OF P]] by auto
+  show "\<forall>a b. app (mk_funrel x P) a b 
+    \<longleftrightarrow> (a \<in> x \<and> P a b \<and> a : BinRelMem \<and> b : BinRelMem)"
+  proof (auto)
+    fix a b assume "app (mk_funrel x P) a b"
+    hence 
+      "a \<in> {a' \<in> x | a' : BinRelMem}" 
+      "b \<in> Repl x (\<lambda>a b. a : BinRelMem \<and> b : BinRelMem \<and> P a b)"
+      "P a b" "a : BinRelMem" "b : BinRelMem"
+      using rel collect_set[OF x, of \<open>\<lambda>a'. a' : BinRelMem\<close>] r_set
+      unfolding mk_funrel_def by auto
+    thus "a \<in> x" "P a b" "a : BinRelMem" "b : BinRelMem"
+       using collectE[OF x] by auto
+  next
+    fix a b assume 
+      "a \<in> x" "P a b" "a : BinRelMem" "b : BinRelMem"
+    moreover hence 
+      "a \<in> {a' \<in> x | a' : BinRelMem}" 
+      "b \<in> Repl x (\<lambda>a b. a : BinRelMem \<and> b : BinRelMem \<and> P a b)"
+      using collectI[OF x] replaceI[OF x frelpred_replpred[OF P] _ _ relmem_setmem] 
+      by auto
+    ultimately show 
+      "app (mk_funrel x P) a b"
+      unfolding mk_funrel_def
+      using rel collect_set[OF x, of \<open>\<lambda>a'. a' : BinRelMem\<close>] r_set by auto
+  qed
 qed
 
 theorem BinRel_Function : 
-  "class.Function Set (\<in>) Union Pow \<emptyset> Succ Inf \<R> (\<subseteq>) SetMem SetOf ReplPred 
-      app FuncRel mk_funrel domain range BinRelMem FuncRelPred"
+  "class.Function_axioms Set (\<in>) app FuncRel mk_funrel domain range BinRelMem FuncRelPred"
 proof (unfold_locales)
-  show "mk_funrel : (\<Pi> x:Set. FuncRelPred x \<rightarrow> FuncRel)" 
-  proof (rule depfunI, rule funI, rule funrelI)
+  show mk_funrel_typ : "mk_funrel : (\<Pi> x:Set. FuncRelPred x \<rightarrow> FuncRel)" 
+  proof (rule depfunI, rule funI, rule funrelI, simp only: mk_funrel_binrel)
     fix x P assume xp:"x : Set" "P : FuncRelPred x"
-    hence "Repl x P : Set" "P : BinRelPred x (Repl x P)"  
-      using repl_set[OF xp(1) frelpred_replpred] frelpred_brelpred by auto
-    thus br:"mk_funrel x P : BinRel" unfolding mk_funrel_def 
-      using mkrel_binrel[OF \<open>x : Set\<close>]  by auto  
-
     show func:"\<forall>a b c. app (mk_funrel x P) a b \<and> app (mk_funrel x P) a c \<longrightarrow> b = c"
     proof (rule)+
       fix a b c assume 
         "app (mk_funrel x P) a b \<and> app (mk_funrel x P) a c"
-      hence "P a b" "P a c" "a \<in> x" "b : BinRelMem" "c : BinRelMem" 
-        using mkfun_rel_iff[OF xp] brelmemI1[OF br] brelmemI2[OF br]  by auto
+      hence "P a b" "P a c" "a \<in> x" "a : BinRelMem" "b : BinRelMem" "c : BinRelMem" 
+        using mkfun_rel_iff[OF xp] by auto
       moreover hence "b : SetMem" "c : SetMem"
         using relmem_setmem by auto
       ultimately show "b = c" 
         using frelpred_replpred[OF \<open>P : FuncRelPred x\<close>]
-        unfolding ReplPred_def has_ty_def tuniq_def Uniq_def by auto
+        unfolding ReplPred_def has_ty_def tuniq_def Uniq_def by auto 
     qed
   qed
 
-  show "domain : FuncRel \<rightarrow> Set" unfolding domain_def 
+  show "domain : FuncRel \<rightarrow> Set" 
+    unfolding domain_def 
   proof (rule funI, rule collect_set)
     fix f assume "f : FuncRel" 
     hence "f : BinRel" unfolding FuncRel_def by (rule intE1)
     thus "field f : Set" by (rule field_set)
   qed
 
-  show "\<forall>s : Set. \<forall>P : FunPred s. \<forall>x y. app (mk_funrel s P) x y = (x \<in> s \<and> P x y)"
-  proof (rule, rule, rule, rule)
-    fix s P x y assume sp: "s : Set" "P : FunPred s" 
-    show "app (mk_funrel s P) x y = (x \<in> s \<and> P x y)" 
-    proof
-      assume "app (mk_funrel s P) x y"
-      thus "x \<in> s \<and> P x y" using mkfun_rel_iff[OF sp] by auto
-    next
-      assume "x \<in> s \<and> P x y"
-      moreover hence "y \<in> Repl s P" 
-        using replaceI[OF \<open>s : Set\<close> funpred_replpred[OF \<open>P : FunPred s\<close>]] by auto
-      ultimately show "app (mk_funrel s P) x y" using mkfun_rel_iff[OF sp] by auto
-    qed
+  show "range : FuncRel \<rightarrow> Set" 
+    unfolding range_def 
+  proof (rule funI, rule collect_set)
+    fix f assume "f : FuncRel" 
+    hence "f : BinRel" unfolding FuncRel_def by (rule intE1)
+    thus "field f : Set" by (rule field_set)
   qed
+
+  show "\<forall>s : Set. \<forall>P : FuncRelPred s. 
+    \<forall>x y. app (mk_funrel s P) x y = (x \<in> s \<and> P x y \<and> x : BinRelMem \<and> y : BinRelMem)"
+    using mkfun_rel_iff by auto
 
   show "\<forall>f : FuncRel. \<forall>x y z. app f x y \<and> app f x z \<longrightarrow> y = z"
     by (rule, unfold FuncRel_def, drule tyE[OF intE2], auto)
@@ -156,13 +187,54 @@ proof (unfold_locales)
   proof (rule, rule)
     fix f x assume "f : FuncRel"
     hence "f : BinRel" unfolding FuncRel_def by (auto elim: intE1)
-    show "(x \<in> domain f) = (\<exists>y. app f x y)" unfolding domain_def collect_iff[OF field_set[OF \<open>f : BinRel\<close>]]
+    show "(x \<in> domain f) = (\<exists>y. app f x y)" 
+      unfolding domain_def collect_iff[OF field_set[OF \<open>f : BinRel\<close>]]
       using field_iff \<open>f : BinRel\<close> by auto
   qed
-qed 
 
-(*Proving that any functional relations can interpret the Function interface!*)
- sorry
+  show "\<forall>f : FuncRel. \<forall>y. (y \<in> range f) = (\<exists>x. app f x y)"
+  proof (rule, rule)
+    fix f y assume "f : FuncRel"
+    hence "f : BinRel" unfolding FuncRel_def by (auto elim: intE1)
+    show "(y \<in> range f) = (\<exists>x. app f x y)" 
+      unfolding range_def collect_iff[OF field_set[OF \<open>f : BinRel\<close>]]
+      using field_iff \<open>f : BinRel\<close> by auto
+  qed
+
+  show "BinRelMem = app_mem FuncRel"
+  proof -
+    have "\<forall>b. b : BinRelMem \<longleftrightarrow> b : app_mem FuncRel"
+    proof (rule)+
+      fix b assume b : "b : BinRelMem"
+      hence b_smem : "b : SetMem" 
+        using relmem_setmem by auto
+      let ?P = "\<lambda>c d. c = b \<and> d = b"
+      have P : "?P : FuncRelPred {b}"
+        unfolding FuncRelPred_def tall_def tuniq_def Uniq_def
+        by (rule tyI, auto)
+      
+      let ?f = "mk_funrel {b} ?P"
+      have "?f : FuncRel" 
+        using funE[OF depfunE[OF mk_funrel_typ 
+              sng_set[OF b_smem]] P] .
+      moreover hence "app ?f b b"
+        using mkfun_rel_iff[OF sng_set[OF b_smem] P] sngI[OF b_smem] b by auto
+      ultimately show "b : app_mem FuncRel"
+        unfolding tex_def has_ty_def by auto
+    next
+      fix b assume "b : app_mem FuncRel"
+      thus "b : BinRelMem"
+        unfolding BinRelMem_def tex_def FuncRel_def inter_ty_def has_ty_def 
+        by auto
+    qed
+    thus ?thesis 
+      unfolding has_ty_def 
+      by presburger
+  qed
+
+  show "FuncRelPred = (\<lambda>s P. \<forall>x : BinRelMem. x \<in> s \<longrightarrow> (\<exists>\<^sub>\<le>\<^sub>1 y : BinRelMem. P x y))"
+    unfolding FuncRelPred_def ..
+qed
 
 end 
 end
